Infra/Bootstrap.v
@@ -1,4 +1,0 @@
-Require Import Arith Coq.Lists.List Setoid Coq.Lists.SetoidList.
-Require Export Infra.Option EqDec AutoIndTac.
-
-Set Implicit Arguments.
